\documentclass{article}
\usepackage{amsmath}
\usepackage{amsfonts}
\usepackage{bm}
\title{EM algorithm}
\author {ywch}
\date{\today}
\begin{document}
\section{EM algorithm}
Likelihood function:
\begin{equation}
    \label{likelihood}
    \mathcal{L}(\Theta) = \Pi_{i=1}^m  \ p(\bm{x}_i,\Theta)
\end{equation}
log likelihood function:
\begin{equation}
    \label{log likelihood}
    \mathcal{L} \mathcal{L}(\Theta) = \sum_{i=1 }^m \log p(\bm{x}_i,\Theta)
\end{equation}
    \begin{align*}
    \mathcal{L} \mathcal{L}(\Theta) & = \sum_{i=1 }^m \log p(\bm{x}_i,\Theta)\\
    & = \sum_{i=1 }^m \log \sum_{\bm{z}_i} p (\bm{x}_i,\bm{z}_i;\Theta) \\
    & = \sum_{i=1 }^m \log \sum_{\bm{z}_i} Q_i(\bm{z}_i) \frac{P(\bm{x}_i,\bm{z}_i;\Theta)}{Q_i(\bm{z}_i)} \\
    & \geq \sum_{i=1 }^m  \sum_{\bm{z}_i} Q_i(\bm{z}_i)  \log   \frac{P(\bm{x}_i,\bm{z}_i;\Theta)}{Q_i(\bm{z}_i)} \\
    \end{align*}
\begin{align*}
     c = &  \frac{p(\bm{x}_i,\bm{z}_i;\Theta)}{Q_i(\bm{z}_i)}  \\
       Q_i(\bm{z}) & = \frac {p(\bm{x}_i,\bm{z}_i;\Theta)}{\sum_{\bm{z}_i}P(\bm{x}_i,\bm{z}_i;\Theta)} \\
        & = \frac {p(\bm{x}_i,\bm{z}_i;\Theta)} {p(\bm{x}_i;\Theta)} \\
      & = p(\bm{z}_i| \bm{x}_i;\Theta) \\
\end{align*}
Repeat until convergence:\\
E-step:
    $$Q_i(\bm{z}_i)=P(\bm{z}_i| \bm{x}_i;\Theta)$$
M-step:
    $$ \arg  \max_{\Theta}  \sum_{i=1 }^m  Q_i(\bm{z}) \log  \sum_{z} \frac{p(\bm{x}_i,\bm{z}_i;\Theta)}{Q_i(\bm{z}_i)} $$
\end{document}